src/ExtractionHaskell/word_by_word_montgomery_generic.v
@@ -1,4 +1,4 @@
 Require Import Crypto.StandaloneHaskellMain.
 
-(*Redirect "/tmp/word_by_word_montgomery.hs" *)Recursive Extraction WordByWordMontgomery.main.
-(* cat /tmp/word_by_word_montgomery.hs.out | sed -f haskell.sed  > ../../word_by_word_montgomery.hs *)
+(*Redirect "/tmp/word_by_word_montgomery_generic.hs" *)Recursive Extraction WordByWordMontgomeryGeneric.main.
+(* cat /tmp/word_by_word_montgomery_generic.hs.out | sed -f haskell.sed  > ../../word_by_word_montgomery_generic.hs *)
