src/StandaloneOCamlMain.v
@@ -194,6 +194,11 @@ Module WordByWordMontgomery.
     := main_gen ForExtraction.WordByWordMontgomery.PipelineMain.
 End WordByWordMontgomery.
 
+Module WordByWordMontgomeryGeneric.
+  Definition main : unit
+    := main_gen ForExtraction.WordByWordMontgomeryGeneric.PipelineMain.
+End WordByWordMontgomeryGeneric.
+
 Module SaturatedSolinas.
   Definition main : unit
     := main_gen ForExtraction.SaturatedSolinas.PipelineMain.
